yalla/fmiformulas.v
@@ -26,13 +26,14 @@ match A with
 | ione => Bnt 2 Lnt Lnt
 | itens A B => Bnt 3 (iform2nattree A) (iform2nattree B)
 | ilpam A B => Bnt 4 (iform2nattree A) (iform2nattree B)
-| ilmap A B => Bnt 5 (iform2nattree A) (iform2nattree B)
-| ineg A => Bnt 6 (iform2nattree A) Lnt
-| itop => Bnt 7 Lnt Lnt
-| iwith A B => Bnt 8 (iform2nattree A) (iform2nattree B)
-| izero => Bnt 9 Lnt Lnt
-| iplus A B => Bnt 10 (iform2nattree A) (iform2nattree B)
-| ioc A => Bnt 11 (iform2nattree A) Lnt
+| igen A => Bnt 5 (iform2nattree A) Lnt
+| ilmap A B => Bnt 6 (iform2nattree A) (iform2nattree B)
+| ineg A => Bnt 7 (iform2nattree A) Lnt
+| itop => Bnt 8 Lnt Lnt
+| iwith A B => Bnt 9 (iform2nattree A) (iform2nattree B)
+| izero => Bnt 10 Lnt Lnt
+| iplus A B => Bnt 11 (iform2nattree A) (iform2nattree B)
+| ioc A => Bnt 12 (iform2nattree A) Lnt
 end.
 
 Fixpoint nattree2iform t :=
@@ -41,13 +42,14 @@ match t with
 | Bnt 2 Lnt Lnt => ione
 | Bnt 3 t1 t2 => itens (nattree2iform t1) (nattree2iform t2)
 | Bnt 4 t1 t2 => ilpam (nattree2iform t1) (nattree2iform t2)
-| Bnt 5 t1 t2 => ilmap (nattree2iform t1) (nattree2iform t2)
-| Bnt 6 t1 Lnt => ineg (nattree2iform t1)
-| Bnt 7 Lnt Lnt => itop
-| Bnt 8 t1 t2 => iwith (nattree2iform t1) (nattree2iform t2)
-| Bnt 9 Lnt Lnt => izero
-| Bnt 10 t1 t2 => iplus (nattree2iform t1) (nattree2iform t2)
-| Bnt 11 t1 Lnt => ioc (nattree2iform t1)
+| Bnt 5 t1 Lnt => igen (nattree2iform t1)
+| Bnt 6 t1 t2 => ilmap (nattree2iform t1) (nattree2iform t2)
+| Bnt 7 t1 Lnt => ineg (nattree2iform t1)
+| Bnt 8 Lnt Lnt => itop
+| Bnt 9 t1 t2 => iwith (nattree2iform t1) (nattree2iform t2)
+| Bnt 10 Lnt Lnt => izero
+| Bnt 11 t1 t2 => iplus (nattree2iform t1) (nattree2iform t2)
+| Bnt 12 t1 Lnt => ioc (nattree2iform t1)
 | _ => ione
 end.
 
